AwsCryptographicMaterialProviders/dafny/AwsCryptographyKeyStoreAdmin/src/InitializeMutation.dfy
@@ -52,6 +52,7 @@ module {:options "/functionSyntax:4" } InternalInitializeMutation {
       && keyManagerStrategy.ValidState()
       && storage.ValidState()
       && SystemKey.Modifies !! keyManagerStrategy.Modifies !! storage.Modifies
+      && keyManagerStrategy.SupportHV1()
     }
   }
 
@@ -118,30 +119,17 @@ module {:options "/functionSyntax:4" } InternalInitializeMutation {
     requires StateStrucs.ValidMutations?(input.Mutations) // may not need this
     requires
       && input.storage.ValidState()
-      && match input.keyManagerStrategy {
-           case reEncrypt(km) => km.kmsClient.ValidState() && AwsKmsUtils.GetValidGrantTokens(Some(km.grantTokens)).Success?
-           case decryptEncrypt(kmD, kmE) =>
-             && kmD.kmsClient.ValidState() && kmE.kmsClient.ValidState()
-             && AwsKmsUtils.GetValidGrantTokens(Some(kmD.grantTokens)).Success?
-             && AwsKmsUtils.GetValidGrantTokens(Some(kmE.grantTokens)).Success?
-         }
+      && input.keyManagerStrategy.ValidState()
       && input.SystemKey.ValidState()
       && input.ValidState()
     ensures
       && input.storage.ValidState()
       && input.SystemKey.ValidState()
-      &&
-         match input.keyManagerStrategy {
-           case reEncrypt(km) => km.kmsClient.ValidState()
-           case decryptEncrypt(kmD, kmE) => kmD.kmsClient.ValidState() && kmE.kmsClient.ValidState()
-         }
+      && input.keyManagerStrategy.ValidState()
       && input.ValidState()
     modifies
       input.storage.Modifies,
-             match input.keyManagerStrategy {
-               case reEncrypt(km) => km.kmsClient.Modifies
-               case decryptEncrypt(kmD, kmE) => kmD.kmsClient.Modifies + kmE.kmsClient.Modifies
-             },
+             input.keyManagerStrategy.Modifies,
              input.SystemKey.Modifies
   {
     var resumeMutation? := false;
@@ -206,6 +194,13 @@ module {:options "/functionSyntax:4" } InternalInitializeMutation {
          ),
       Types.KeyStoreAdminException(
         message := "Active Branch Key Item read from storage is malformed!")
+    );
+
+      // TODO-HV-2-M2: Support items in HV-2
+    :- Need(
+      readItems.ActiveItem.EncryptionContext[Structure.HIERARCHY_VERSION] == Structure.HIERARCHY_VERSION_VALUE_1,
+      Types.KeyStoreAdminException(
+        message := "At this time, Mutations ONLY support HV-1; BK's Active Item is HV-2.")
     );
 
     :- Need(
@@ -390,10 +385,8 @@ module {:options "/functionSyntax:4" } InternalInitializeMutation {
                KeyStoreTypes.kmsKeyArn(mutationToApply.Terminal.kmsArn), decryptOnlyEncryptionContext
              )
     requires keyManagerStrategy.ValidState()
-    modifies
-      match keyManagerStrategy
-      case reEncrypt(kms) => kms.kmsClient.Modifies
-      case decryptEncrypt(kmsD, kmsE) => kmsD.kmsClient.Modifies + kmsE.kmsClient.Modifies
+    requires keyManagerStrategy.SupportHV1()
+    modifies keyManagerStrategy.Modifies
     ensures keyManagerStrategy.ValidState()
     ensures res.Success? ==>
               && Structure.BranchKeyContext?(res.value.EncryptionContext)
@@ -573,13 +566,11 @@ module {:options "/functionSyntax:4" } InternalInitializeMutation {
       && 0 < |input.Identifier|
       && activeItem.KmsArn == mutationToApply.Original.kmsArn
       && Structure.EncryptedHierarchicalKey?(activeItem)
+      && input.keyManagerStrategy.SupportHV1()
     }
 
     ghost const Modifies :=
-      match input.keyManagerStrategy {
-        case reEncrypt(km) => multiset(km.kmsClient.Modifies)
-        case decryptEncrypt(kmD, kmE) => multiset(kmD.kmsClient.Modifies) + multiset(kmE.kmsClient.Modifies)
-      }
+      input.keyManagerStrategy.ModifiesMultiSet
       + multiset(input.SystemKey.Modifies)
       + multiset(input.storage.Modifies)
   }
